

On the Sum $\sum_{n=1}^i \frac{n(n+1)\dots(n+a)}{(a+1)!}$

Akash Pardeshi

University of Illinois Laboratory High School

September 2017

Introduction

In this paper, I will prove the following:

$$\sum_{n=1}^i \frac{n(n+1)\dots(n+a)}{(a+1)!} = \frac{i(i+1)\dots(i+a)(i+a+1)}{(a+2)!}.$$

Preparatory Proofs

Before we can prove this, we must show a few other things, starting with

$$\begin{aligned} \sum_{n=1}^i \frac{n(n+1)\dots(n+a)}{(a+1)!} &= \sum_{n=1}^1 \frac{n(n+1)\dots(n+a-1)}{a!} + \sum_{n=1}^2 \frac{n(n+1)\dots(n+a-1)}{a!} + \dots + \\ &\quad \sum_{n=1}^{i-1} \frac{n(n+1)\dots(n+a-1)}{a!} + \sum_{n=1}^i \frac{n(n+1)\dots(n+a-1)}{a!}. \end{aligned} \quad (1)$$

If we write each of the terms on the RHS in closed form we get

$$\begin{aligned} \sum_{n=1}^i \frac{n(n+1)\dots(n+a)}{(a+1)!} &= \frac{1(2)\dots(1+a-1)(1+a)}{(a+1)!} + \frac{2(3)\dots(2+a-1)(2+a)}{(a+1)!} + \dots + \\ &\quad \frac{(i-1)(i)\dots(i+a-1)(i+a)}{(a+1)!} + \frac{i(i+1)\dots(i+a-1)(i+a)}{(a+1)!}. \end{aligned}$$

The RHS is the written out expansion of the sum on the LHS so our original claim is true. From this, we can also say that

$$\begin{aligned} \sum_{n=1}^i \frac{n(n+1)\dots(n+a)}{(a+1)!} &= \sum_{n=1}^1 \frac{n(n+1)\dots(n+a-1)}{a!} + \sum_{n=1}^2 \frac{n(n+1)\dots(n+a-1)}{a!} + \dots + \\ &\quad \sum_{n=1}^{i-1} \frac{n(n+1)\dots(n+a-1)}{a!} + \sum_{n=1}^i \frac{n(n+1)\dots(n+a-1)}{a!} \\ \sum_{n=1}^i \frac{n(n+1)\dots(n+a)}{(a+1)!} &= \sum_{n=1}^{i-1} \frac{n(n+1)\dots(n+a)}{(a+1)!} + \sum_{n=1}^i \frac{n(n+1)\dots(n+a-1)}{a!}. \end{aligned} \quad (2)$$

If we apply the expansion from 1 to each term in the expansion, we get

$$\begin{aligned} \sum_{n=1}^i \frac{n(n+1)\dots(n+a)}{(a+1)!} &= \left(\sum_{n=1}^1 \frac{n(n+1)\dots(n+a-2)}{(a-1)!} \right) + \left(\sum_{n=1}^1 \frac{n(n+1)\dots(n+a-2)}{(a-1)!} + \sum_{n=1}^2 \frac{n(n+1)\dots(n+a-2)}{(a-1)!} \right) + \dots + \\ &\left(\sum_{n=1}^1 \frac{n(n+1)\dots(n+a-2)}{(a-1)!} + \sum_{n=1}^2 \frac{n(n+1)\dots(n+a-2)}{(a-1)!} + \dots + \sum_{n=1}^{i-1} \frac{n(n+1)\dots(n+a-2)}{(a-1)!} \right) + \\ &\left(\sum_{n=1}^1 \frac{n(n+1)\dots(n+a-2)}{(a-1)!} + \sum_{n=1}^2 \frac{n(n+1)\dots(n+a-2)}{(a-1)!} + \dots + \sum_{n=1}^i \frac{n(n+1)\dots(n+a-2)}{(a-1)!} \right). \end{aligned}$$

We can factor this expression by realizing that all i terms contain the term,

$$\sum_{n=1}^1 \frac{n(n+1)\dots(n+a-2)}{(a-1)!}$$

$i-1$ terms contain the term,

$$\sum_{n=1}^2 \frac{n(n+1)\dots(n+a-2)}{(a-1)!}$$

and only the final term contains the term

$$\sum_{n=1}^i \frac{n(n+1)\dots(n+a-2)}{(a-1)!}.$$

Thus, the factored form is

$$i \sum_{n=1}^1 \frac{n(n+1)\dots(n+a-2)}{(a-1)!} + (i-1) \sum_{n=1}^2 \frac{n(n+1)\dots(n+a-2)}{(a-1)!} + \dots + 1 \sum_{n=1}^i \frac{n(n+1)\dots(n+a-2)}{(a-1)!}. \quad (3)$$

If we repeat this process, we would get $1 \sum_{n=1}^i \frac{n(n+1)\dots(n+a-3)}{(a-2)!}$ terms in the first grouping, 2 in the second, and i in the last. Similarly, there would be $1 \sum_{n=1}^{i-1} \frac{n(n+1)\dots(n+a-3)}{(a-2)!}$ in the second grouping, and $i-1$ in the last. If we carry this process on for all terms, we arrive at the factorization

$$\begin{aligned} \sum_{n=1}^i \frac{n(n+1)\dots(n+a-3)}{(a-2)!} &= \left(\sum_{n=1}^i n \right) \left(\sum_{n=1}^1 \frac{n(n+1)\dots(n+a-3)}{(a-2)!} \right) + \left(\sum_{n=1}^{i-1} n \right) \left(\sum_{n=1}^2 \frac{n(n+1)\dots(n+a-3)}{(a-2)!} \right) + \dots + \\ &\left(\sum_{n=1}^1 n \right) \left(\sum_{n=1}^i \frac{n(n+1)\dots(n+a-3)}{(a-2)!} \right). \quad (4) \end{aligned}$$

With these tools, we can now prove our theorem.

Proof

We start by writing out our sum

$$\sum_{n=1}^i \frac{n(n+1)\dots(n+a)}{(a+1)!} = \frac{1(2)\dots(a-1)(a)(a+1)}{(a+1)!} + \frac{2(3)\dots(a)(a+1)(a+2)}{(a+1)!} + \dots + \frac{i(i+1)\dots(i+a-1)(i+a)(i+a+1)}{(a+1)!}.$$

We can re-write the last two factors in each term with $i + a$ as such

$$\sum_{n=1}^i \frac{n(n+1)\dots(n+a)}{(a+1)!} = \frac{1(2)\dots(a-1)((i+a)-i)((i+a)-(i-1))}{(a+1)!} + \frac{2(3)\dots(a)((i+a)-(i-1))((i+a)-(i-2))}{(a+1)!} + \dots + \frac{i(i+1)\dots(i+a-2)((i+a)-1)(i+a)}{(a+1)!}.$$

We can re-write this as

$$\begin{aligned} (a+1)! \sum_{n=1}^i \frac{n(n+1)\dots(n+a)}{(a+1)!} &= (a-1)! \frac{1(2)\dots(a-1)}{(a-1)!} ((i+a)-i)((i+a)-(i-1)) + \\ &\quad (a-1)! \frac{2(3)\dots(a)}{(a-1)!} ((i+a)-(i-1))((i+a)-(i-2)) + \dots + \\ &\quad (a-1)! \frac{i(i+1)\dots(i+a-2)}{(a-1)!} ((i+a)-1)(i+a) \end{aligned}$$

Using the statement we are trying to prove to simplify

$$\begin{aligned} (a+1)! \sum_{n=1}^i \frac{n(n+1)\dots(n+a)}{(a+1)!} &= (a-1)! \sum_{n=1}^1 \frac{n(n+1)\dots(n+a-3)}{(a-2)!} ((i+a)-i)((i+a)-(i-1)) + \\ &\quad (a-1)! \sum_{n=1}^2 \frac{n(n+1)\dots(n+a-3)}{(a-2)!} ((i+a)-(i-1))((i+a)-(i-2)) + \dots + \\ &\quad (a-1)! \sum_{n=1}^{i-1} \frac{n(n+1)\dots(n+a-3)}{(a-2)!} ((i+a)-2)((i+a)-1) + \\ &\quad (a-1)! \sum_{n=1}^i \frac{n(n+1)\dots(n+a-3)}{(a-2)!} ((i+a)-1)(i+a). \end{aligned}$$

Multiplying the binomials

$$\begin{aligned} (a+1)! \sum_{n=1}^i \frac{n(n+1)\dots(n+a)}{(a+1)!} &= (a-1)! \sum_{n=1}^1 \frac{n(n+1)\dots(n+a-3)}{(a-2)!} ((i+a)^2 - i(i+a) - (i-1)(i+a) + (i-1)i) + \\ &\quad (a-1)! \sum_{n=1}^2 \frac{n(n+1)\dots(n+a-3)}{(a-2)!} ((i+a)^2 - (i+a)(i-1) - (i-a)(i-2) + (i-2)(i-2)) + \dots + \\ &\quad (a-1)! \sum_{n=1}^{i-1} \frac{n(n+1)\dots(n+a-3)}{(a-2)!} ((i+a)^2 - 2(i+a) - 1(i+a) + 1(2)) + \\ &\quad (a-1)! \sum_{n=1}^i \frac{n(n+1)\dots(n+a-3)}{(a-2)!} ((i+a)^2 - 1(i+a)). \end{aligned}$$

Combining the first terms of each grouping

$$\begin{aligned}
(a+1)! \sum_{n=1}^i \frac{n(n+1)\dots(n+a)}{(a+1)!} &= (a-1)!(i+a)^2 \left(\sum_{n=1}^1 \frac{n(n+1)\dots(n+a-3)}{(a-2)!} + \sum_{n=1}^2 \frac{n(n+1)\dots(n+a-3)}{(a-2)!} + \dots + \right. \\
&\sum_{n=1}^i \frac{n(n+1)\dots(n+a-3)}{(a-2)!} \Big) - (a-1)!(i+a) \left(i \sum_{n=1}^1 \frac{n(n+1)\dots(n+a-3)}{(a-2)!} + (i-1) \sum_{n=1}^2 \frac{n(n+1)\dots(n+a-3)}{(a-2)!} + \dots + \right. \\
&2 \sum_{n=1}^{i-1} \frac{n(n+1)\dots(n+a-3)}{(a-2)!} + 1 \sum_{n=1}^i \frac{n(n+1)\dots(n+a-3)}{(a-2)!} \Big) - (a-1)!(i+a) \\
&\left((i-1) \sum_{n=1}^1 \frac{n(n+1)\dots(n+a-3)}{(a-2)!} + (i-2) \sum_{n=1}^2 \frac{n(n+1)\dots(n+a-3)}{(a-2)!} + \dots + \right. \\
&2 \sum_{n=1}^{i-2} \frac{n(n+1)\dots(n+a-3)}{(a-2)!} + 1 \sum_{n=1}^{i-1} \frac{n(n+1)\dots(n+a-3)}{(a-2)!} \Big) + (a-1)! \left((i-1)i \sum_{n=1}^{i-1} \frac{n(n+1)\dots(n+a-3)}{(a-2)!} \right. \\
&\left. + (i-2)(i-1) \sum_{n=1}^{i-2} \frac{n(n+1)\dots(n+a-3)}{(a-2)!} + \dots + 1(2) \sum_{n=1}^1 \frac{n(n+1)\dots(n+a-3)}{(a-2)!} \right).
\end{aligned}$$

By our previous observations in equations 1, 3, and 4, we can say

$$\begin{aligned}
(a+1)! \sum_{n=1}^i \frac{n(n+1)\dots(n+a)}{(a+1)!} &= (a-1)!(i+a)^2 \left(\sum_{n=1}^i \frac{n(n+1)\dots(n+a-2)}{(a-1)!} \right) - (a-1)!(i+a) \sum_{n=1}^i \frac{n(n+1)\dots(n+a-1)}{a!} \\
&- (a-1)!(i+a) \sum_{n=1}^{i-1} \frac{n(n+1)\dots(n+a-1)}{a!} + (a-1)! \cdot 2! \left(\sum_{n=1}^{i-1} \frac{n(n+1)\dots(n+a)}{(a+1)!} \right).
\end{aligned}$$

By equation 2, we can rewrite the equation as

$$\begin{aligned}
(a+1)! \sum_{n=1}^{i-1} \frac{n(n+1)\dots(n+a)}{(a+1)!} + (a+1)! \sum_{n=1}^i \frac{n(n+1)\dots(n+a-1)}{a!} &= (a-1)!(i+a)^2 \left(\sum_{n=1}^i \frac{n(n+1)\dots(n+a-2)}{(a-1)!} \right) \\
- (a-1)!(i+a) \left(\sum_{n=1}^i \frac{n(n+1)\dots(n+a-1)}{a!} + \sum_{n=1}^{i-1} \frac{n(n+1)\dots(n+a-1)}{a!} \right) &+ (a-1)! \cdot 2! \left(\sum_{n=1}^{i-1} \frac{n(n+1)\dots(n+a)}{(a+1)!} \right).
\end{aligned}$$

Further expanding the equation

$$\begin{aligned}
(a+1)! \sum_{n=1}^{i-1} \frac{n(n+1)\dots(n+a)}{(a+1)!} + (a+1)! \sum_{n=1}^{i-1} \frac{n(n+1)\dots(n+a-1)}{a!} &+ (a+1)! \sum_{n=1}^i \frac{n(n+1)\dots(n+a-2)}{(a-1)!} = \\
(a-1)!(i+a)^2 \sum_{n=1}^i \frac{n(n+1)\dots(n+a-2)}{(a-1)!} - (a-1)!(i+a) \left(\sum_{n=1}^{i-1} \frac{n(n+1)\dots(n+a-1)}{a!} + \right. \\
\left. \sum_{n=1}^i \frac{n(n+1)\dots(n+a-2)}{(a-1)!} + \sum_{n=1}^{i-1} \frac{n(n+1)\dots(n+a-1)}{a!} \right) &+ (a-1)! \cdot 2! \left(\sum_{n=1}^{i-1} \frac{n(n+1)\dots(n+a)}{(a+1)!} \right).
\end{aligned}$$

Combining like terms

$$\begin{aligned}
& \left((a+1)! - 2!(a-1)! \right) \sum_{n=1}^{i-1} \frac{n(n+1)\dots(n+a)}{(a+1)!} + (a+1)! \sum_{n=1}^{i-1} \frac{n(n+1)\dots(n+a-1)}{a!} + (a+1)! \sum_{n=1}^i \frac{n(n+1)\dots(n+a-2)}{(a-1)!} = \\
& (a-1)!(i+a)^2 \sum_{n=1}^i \frac{n(n+1)\dots(n+a-2)}{(a-1)!} - (a-1)!(i+a) \left(2 \sum_{n=1}^{i-1} \frac{n(n+1)\dots(n+a-1)}{a!} + \sum_{n=1}^i \frac{n(n+1)\dots(n+a-2)}{(a-1)!} \right) \\
& \left((a+1)! - 2!(a-1)! \right) \sum_{n=1}^{i-1} \frac{n(n+1)\dots(n+a)}{(a+1)!} + (a+1)! \sum_{n=1}^{i-1} \frac{n(n+1)\dots(n+a-1)}{a!} + (a+1)! \sum_{n=1}^i \frac{n(n+1)\dots(n+a-2)}{(a-1)!} = \\
& (a-1)!(i+a)^2 \sum_{n=1}^i \frac{n(n+1)\dots(n+a-2)}{(a-1)!} - (a-1)!2(i+a) \sum_{n=1}^{i-1} \frac{n(n+1)\dots(n+a-1)}{a!} - (a-1)!(i+a) \sum_{n=1}^i \frac{n(n+1)\dots(n+a-2)}{(a-1)!}
\end{aligned}$$

Factoring

$$\begin{aligned}
& \left((a+1)! - 2!(a-1)! \right) \sum_{n=1}^{i-1} \frac{n(n+1)\dots(n+a)}{(a+1)!} = \\
& \left((a-1)!(i+a)^2 - (a-1)!(i+a) - (a+1)! \right) \sum_{n=1}^i \frac{n(n+1)\dots(n+a-2)}{(a-1)!} - \left((a-1)!2(i+a) + (a+1)! \right) \sum_{n=1}^{i-1} \frac{n(n+1)\dots(n+a-1)}{a!}.
\end{aligned}$$

Factoring an $(a-1)!$ out of all terms

$$\begin{aligned}
& (a-1)!(a(a+1) - 2!) \sum_{n=1}^{i-1} \frac{n(n+1)\dots(n+a)}{(a+1)!} = \\
& (a-1)! \left((i+a)^2 - (i+a) - a(a+1) \right) \sum_{n=1}^i \frac{n(n+1)\dots(n+a-2)}{(a-1)!} - (a-1)! \left(2(i+a) + a(a+1) \right) \sum_{n=1}^{i-1} \frac{n(n+1)\dots(n+a-1)}{a!}
\end{aligned}$$

Dividing by $(a-1)!$

$$\begin{aligned}
& (a(a+1) - 2!) \sum_{n=1}^{i-1} \frac{n(n+1)\dots(n+a)}{(a+1)!} = \\
& \left((i+a)^2 - (i+a) - a(a+1) \right) \sum_{n=1}^i \frac{n(n+1)\dots(n+a-2)}{(a-1)!} - \left(2(i+a) + a(a+1) \right) \sum_{n=1}^{i-1} \frac{n(n+1)\dots(n+a-1)}{a!} \\
& (a^2 + a - 2) \sum_{n=1}^{i-1} \frac{n(n+1)\dots(n+a)}{(a+1)!} = \\
& \left(i^2 + 2ai + a^2 - i - a - a^2 - a \right) \sum_{n=1}^i \frac{n(n+1)\dots(n+a-2)}{(a-1)!} - \left(2i + 2a + a^2 + a \right) \sum_{n=1}^{i-1} \frac{n(n+1)\dots(n+a-1)}{a!} \\
& (a+2)(a-1) \sum_{n=1}^{i-1} \frac{n(n+1)\dots(n+a)}{(a+1)!} = \\
& \left(i^2 + 2ai - i - 2a \right) \sum_{n=1}^i \frac{n(n+1)\dots(n+a-2)}{(a-1)!} - \left(2i + 3a + a^2 \right) \sum_{n=1}^{i-1} \frac{n(n+1)\dots(n+a-1)}{a!}.
\end{aligned}$$

Factoring

$$(a+2)(a-1) \sum_{n=1}^{i-1} \frac{n(n+1)\dots(n+a)}{(a+1)!} =$$

$$\left(i(i-1) + 2a(i-1) \right) \sum_{n=1}^i \frac{n(n+1)\dots(n+a-2)}{(a-1)!} - \left(2i-2+3a+a^2+2 \right) \sum_{n=1}^{i-1} \frac{n(n+1)\dots(n+a-1)}{a!}$$

$$(a+2)(a-1) \sum_{n=1}^{i-1} \frac{n(n+1)\dots(n+a)}{(a+1)!} =$$

$$\left((i-1)(i+2a) \right) \sum_{n=1}^i \frac{n(n+1)\dots(n+a-2)}{(a-1)!} - \left(2(i-1) + (a+1)(a+2) \right) \sum_{n=1}^{i-1} \frac{n(n+1)\dots(n+a-1)}{a!}$$

Splitting the last term

$$(a+2)(a-1) \sum_{n=1}^{i-1} \frac{n(n+1)\dots(n+a)}{(a+1)!} =$$

$$(i-1)(i+2a) \sum_{n=1}^i \frac{n(n+1)\dots(n+a-2)}{(a-1)!} - (a+1)(a+2) \sum_{n=1}^{i-1} \frac{n(n+1)\dots(n+a-1)}{a!} - 2(i-1) \sum_{n=1}^{i-1} \frac{n(n+1)\dots(n+a-1)}{a!}$$

Writing each term in its closed form

$$(a+2)(a-1) \sum_{n=1}^{i-1} \frac{n(n+1)\dots(n+a)}{(a+1)!} = (i-1)(i+2a) \frac{i(i+1)\dots(i+a-2)(i+a-1)}{a!}$$

$$- (a+1)(a+2) \frac{(i-1)i\dots(i+a-2)(i+a-1)}{(a+1)!} - 2(i-1) \frac{(i-1)i\dots(i+a-2)(i+a-1)}{(a+1)!}$$

$$(a+2)(a-1) \sum_{n=1}^{i-1} \frac{n(n+1)\dots(n+a)}{(a+1)!} = \frac{(i-1)i\dots(i+a-1)}{(a+1)!} \left((i+2a)(a+1) - (a+1)(a+2) - 2(i-1) \right)$$

$$(a+2)(a-1) \sum_{n=1}^{i-1} \frac{n(n+1)\dots(n+a)}{(a+1)!} = \frac{(i-1)i\dots(i+a-1)}{(a+1)!} \left(ai + 2a^2 + i + 2a - a^2 - 3a - 2 - 2i + 2 \right)$$

$$(a+2)(a-1) \sum_{n=1}^{i-1} \frac{n(n+1)\dots(n+a)}{(a+1)!} = \frac{(i-1)i\dots(i+a-1)}{(a+1)!} \left(ai + a^2 - a - i \right)$$

$$(a+2)(a-1) \sum_{n=1}^{i-1} \frac{n(n+1)\dots(n+a)}{(a+1)!} = \frac{(i-1)i\dots(i+a-1)}{(a+1)!} \left(a(i+a) - (i+a) \right)$$

$$(a+2)(a-1) \sum_{n=1}^{i-1} \frac{n(n+1)\dots(n+a)}{(a+1)!} = \frac{(i-1)i\dots(i+a-1)}{(a+1)!} (a-1)(i+a)$$

$$(a+2) \sum_{n=1}^{i-1} \frac{n(n+1)\dots(n+a)}{(a+1)!} = \frac{(i-1)i\dots(i+a-1)}{(a+1)!} (i+a)$$

$$\boxed{\sum_{n=1}^{i-1} \frac{n(n+1)\dots(n+a)}{(a+1)!} = \frac{(i-1)i\dots(i+a-1)(i+a)}{(a+2)!}}$$